fstar/PPP.fst
@@ -1,0 +1,696 @@
+module PPP
+
+open FStar.Tactics
+open Hacspec.Lib
+open FStar.Mul
+open Hacspec.Chacha20
+
+module S = Spec.Chacha20
+module H = Hacspec.Chacha20
+module Seq = Lib.Sequence
+
+module LC = Lib.LoopCombinators
+
+#set-options "--fuel 0 --ifuel 0 --z3rlimit 30"
+
+let equiv_line (a b d: state_idx_t) (s: pos {s < 32}) (state: state_t)
+  : Lemma (S.line a b d (pub_u32 s) state == H.chacha20_line a b d s state)
+          [SMTPat (H.chacha20_line a b d s state)]
+  = assert (S.line a b d (pub_u32 s) state `Seq.equal` H.chacha20_line a b d s state)
+
+let equiv_constants_init
+  : squash (Lib.Sequence.map secret S.chacha20_constants == chacha20_constants_init ())
+  = let l = S.([c0;c1;c2;c3]) in
+    assert_norm (FStar.List.Tot.length l == 4);
+    assert_norm S.(let h (i:nat{i<4}) = FStar.List.Tot.index l i in h 0 = c0 /\ h 1 = c1 /\ h 2 = c2 /\ h 3 = c3);
+    Lib.Sequence.eq_intro (Lib.Sequence.map #_ #_ #(4 <: size_nat) secret S.chacha20_constants) (chacha20_constants_init ())
+
+let equiv_init (key: cha_cha_key_t) (iv: cha_cha_iv_t) (ctr: uint32)
+  : Lemma (S.chacha20_init key iv (v ctr) == H.chacha20_init key iv ctr)
+          [SMTPat (chacha20_init key iv ctr)]
+  = ()
+
+let equiv_quarter_round (a b c d: state_idx_t) (state: state_t)
+  : Lemma (S.quarter_round a b c d state == H.chacha20_quarter_round a b c d state)
+          [SMTPat (chacha20_quarter_round a b c d state)]
+  = ()
+
+let equiv_double_round (state: state_t)
+  : Lemma (S.double_round state == H.chacha20_double_round state)
+          [SMTPat (H.chacha20_double_round state)]
+  = ()
+
+
+let rec make_list (elem: 'a) (n: nat): list 'a
+  = if n = 0 then [] else elem::make_list elem (n-1)
+
+let unfold_foldi (lo: uint_size) (hi: uint_size{lo <= hi})
+                 (f: (i:uint_size{i < hi}) -> 'a -> 'a)
+                 (init: 'a)
+  : Lemma (foldi lo hi f init == (if lo = hi then init else
+                                 foldi (lo + 1) hi f (f lo init)))
+  = assert_norm ((foldi lo hi f init == (if lo = hi then init else
+                                 foldi (lo + 1) hi f (f lo init))))
+
+
+let unfold_repeat (f: 'a -> 'a) (acc0: 'a) (i:pos)
+  : Lemma (LC.repeat i f acc0 == f (LC.repeat (i - 1) f acc0))
+  = LC.unfold_repeat i f acc0 (i-1) 
+
+let eq_foldi0 (hi: uint_size) (f: (i:uint_size{i < hi}) -> 'a -> 'a) (init: 'a)
+  : Lemma (foldi hi hi f init == init)
+  = assert_norm (foldi hi hi f init == init)
+
+#push-options "--max_fuel 0 --z3rlimit 15"
+let equiv_rounds (st: state_t)
+  : Lemma (S.rounds st == H.chacha20_rounds st)
+          [SMTPat (H.chacha20_rounds st)]
+  = assert (S.rounds st == chacha20_rounds st) 
+        by (norm [delta_only [`%S.rounds; `%chacha20_rounds]];
+            iter (fun _ -> l_to_r [`unfold_repeat]) (make_list () 10);
+            l_to_r [`LC.eq_repeat0];
+            norm [primops; iota; delta_only [`%usize; `%foldi]; zeta_full])
+#pop-options
+
+let equiv_core (ctr: uint32) (st0: state_t)
+  : Lemma (S.chacha20_core (v ctr) st0 == chacha20_core ctr st0)
+          [SMTPat (chacha20_core ctr st0)]
+  = let s0 = st0 in
+    let s1 = array_upd st0 (usize 12) (
+                      (array_index (s0) (usize 12)) +. (ctr)) in
+    let k = H.chacha20_rounds s1 in
+    let ka = k `array_add (+.)` s1 in
+    let kb = k `array_add (+.)` s0 in
+    let kb' = array_upd kb (usize 12) (
+                      (array_index (kb) (usize 12)) +. (ctr)) in
+    assert (u32 (v ctr) == ctr);
+    assert(S.chacha20_add_counter s0 (v ctr) == s1);
+    assert(S.rounds s1 == H.chacha20_rounds s1);
+    assert(S.sum_state k s0 == kb);
+    assert(S.chacha20_add_counter kb (v ctr) == kb');
+    assert(ka == H.chacha20_core ctr st0);
+    assert(kb' == S.chacha20_core (v ctr) st0);
+    assert(forall i. i <> 12 ==> s0.[i] ==  s1.[i]);
+    assert(forall i. i <> 12 ==> ka.[i] ==  kb.[i]);
+    assert(forall i. i <> 12 ==> ka.[i] ==  kb'.[i]);
+    assert(s1.[12] ==  s0.[12] +. ctr);
+    assert(ka.[12] ==  k.[12] +. s1.[12]);
+    assert(kb.[12] ==  k.[12] +. s0.[12]);
+    assert(kb'.[12] ==  k.[12] +. s0.[12] +. ctr);
+    assert(kb'.[12] ==  k.[12] +. (s0.[12] +. ctr));
+    assert(kb'.[12] ==  k.[12] +. s1.[12]);
+    assert(forall i. i >= 0 /\ i < 16 ==> ka.[i] ==  kb'.[i]);
+    Lib.Sequence.eq_intro ka kb'
+
+let equiv_key_block (state: state_t)
+  : Lemma (S.chacha20_key_block state == chacha20_key_block state)
+          [SMTPat (chacha20_key_block state)]
+  = ()
+
+let equiv_key_block0 (key: cha_cha_key_t) (iv: cha_cha_iv_t)
+  : Lemma (chacha20_key_block0 key iv == S.chacha20_key_block0 key iv)
+          [SMTPat (chacha20_key_block0 key iv)]
+  = ()
+
+let equiv_encrypt_block (st0: state_t) (ctr: uint32) (plain: block_t)
+  : Lemma (H.chacha20_encrypt_block st0 ctr plain == S.chacha20_encrypt_block st0 (v ctr) plain)
+          [SMTPat (chacha20_encrypt_block st0 ctr plain)]
+  = ()
+
+let equiv_encrypt_last (st0:state_t) (ctr:uint32) (plain: byte_seq {seq_len plain < 64})
+  : Lemma (H.chacha20_encrypt_last st0 ctr plain == S.chacha20_encrypt_last st0 (v ctr) (seq_len plain) plain)
+          [SMTPat (H.chacha20_encrypt_last st0 ctr plain)]
+  = ()
+
+let s_chacha20_update (ctx: S.state) (cipher: seq (int_t U8 SEC)): seq _ =
+  Lib.Sequence.map_blocks 64 cipher
+    (S.chacha20_encrypt_block ctx)
+    (S.chacha20_encrypt_last ctx)
+
+  // (f:(Seq.block (Seq.length input) blocksize -> lseq 'a blocksize -> lseq 'a blocksize))
+  // (g:(Seq.last (Seq.length input) blocksize -> rem:size_nat{rem < blocksize} -> s:lseq 'a rem -> lseq 'a rem))
+
+module IC = IndexableContent
+
+#push-options "--ifuel 0 --z3rlimit 4"
+let map_blocks_pointwise_spec'
+  (len: uint_size)
+  (limit: uint_size {limit <= len})
+  (blocksize: size_pos)
+  (blocks: Seq.block len blocksize -> lseq 'a blocksize)
+  (last_block: lseq 'a (len % blocksize))
+  (output: lseq 'a len)
+  = let last_block_n = len / blocksize in
+    forall (i:nat {i < limit}).
+      let block_n = i / blocksize in
+      let local_i = i % blocksize in
+      assert (i < len);
+      IC.division_order_lemma_ge len i blocksize;
+      assert (block_n <= last_block_n);
+      ( if block_n = last_block_n
+        then let local_i: i:nat {i < len % blocksize} = local_i in
+             Seq.index last_block local_i
+        else Seq.index (blocks block_n) local_i
+      ) == Seq.index output i
+#pop-options
+
+let map_blocks_pointwise_spec'0
+  (len: uint_size)
+  (blocksize: size_pos)
+  (blocks: Seq.block len blocksize -> lseq 'a blocksize)
+  (last_block: lseq 'a (len % blocksize))
+  (output: lseq 'a len)
+  : Lemma (map_blocks_pointwise_spec' len 0 blocksize blocks last_block output)
+  = ()
+
+
+let map_blocks_pointwise_spec
+  (len: uint_size)
+  (blocksize: size_pos)
+  (blocks: Seq.block len blocksize -> lseq 'a blocksize)
+  (last_block: lseq 'a (len % blocksize))
+  (output: lseq 'a len)
+  = map_blocks_pointwise_spec' len len blocksize blocks last_block output
+
+
+#push-options "--z3rlimit 30"
+let sub_rem_lemma (a b: nat) (k: pos)
+  : Lemma (requires (a + 1) * k > b /\ a * k < b)
+          (ensures  b - a * k == b % k)
+  = assert ((a + 1) * k > b);
+    let kb, rb = b / k, b % k in
+    Math.Lemmas.euclidean_division_definition b k;
+    Math.Lemmas.small_div rb k;
+    if kb > a
+    then (
+      IC.division_order_lemma_gt (a + 1) (kb * k + rb) k
+    ) else if kb < a then (
+      IC.division_order_lemma_gt (k * kb + rb) (a * k) k;
+      Math.Lemmas.cancel_mul_div  a k;
+      Math.Lemmas.cancel_mul_div kb k
+    )
+#pop-options
+
+#push-options "--z3rlimit 100"
+let seq_get_remainder_chunk_length_lemma (inp:seq 'a) (blocksize:size_pos)
+  : Lemma (Seq.length (seq_get_remainder_chunk inp blocksize) == Seq.length inp % blocksize)
+  = let r = seq_get_remainder_chunk inp blocksize in
+    let chunks = seq_num_chunks inp blocksize in
+    let last_chunk = if chunks > 0 then chunks - 1 else 0 in
+    assert (seq_chunk_len inp blocksize last_chunk == (
+      if blocksize * (last_chunk + 1) > Seq.length inp
+      then (if blocksize * last_chunk < Seq.length inp
+            then sub_rem_lemma last_chunk (Seq.length inp) blocksize;
+            Seq.length inp % blocksize)
+      else blocksize
+    ));
+    let (_, chunk) = seq_get_chunk inp blocksize last_chunk in
+    if Seq.length chunk = blocksize
+    then Math.Lemmas.cancel_mul_mod (last_chunk + 1) blocksize
+#pop-options
+
+// let map_blocks_foldi'
+//     (#len: uint_size) (blen:uint_size) (lo: uint_size) (hi: uint_size {hi * blen <= len /\ lo <= hi})
+//     (f: (i:uint_size{i < hi}) -> lseq 'a blen) (s: lseq 'a len)
+//     : lseq 'a len
+//   = foldi lo hi (fun i (s: lseq 'a len) -> seq_set_exact_chunk #_ #len s blen i (f i)) s
+
+#push-options "--z3rlimit 150"
+let map_blocks_f_equiv_lemma
+  (len: uint_size) (blocksize: size_pos)
+  (max: uint_size {max * blocksize <= len})
+  (original_s: lseq 'a len)
+  (f:(i:nat{i < max}) -> lseq 'a blocksize -> lseq 'a blocksize)
+  (i: nat{i < max})
+  (updated_s: lseq 'a len {forall (j:nat{j >= i * blocksize /\ j < len}). FStar.Seq.index original_s j == FStar.Seq.index updated_s j})
+  (acc: lseq 'a (i * blocksize) {forall (j:nat{j < i * blocksize}). FStar.Seq.index acc j == FStar.Seq.index updated_s j})
+  // (acc: lseq 'a (i * blocksize) {acc == FStar.Seq.slice updated_s 0 (i * blocksize)})
+  : Lemma (
+          let slice_s = FStar.Seq.slice original_s 0 (max * blocksize) in
+          forall (j: nat{j < (i+1) * blocksize}).
+            FStar.Seq.index (Seq.map_blocks_f blocksize max slice_s f i acc) j
+         == FStar.Seq.index (seq_set_exact_chunk #_ #len updated_s blocksize i (f i (seq_get_exact_chunk updated_s blocksize i))) j
+    )
+  = let slice_s = FStar.Seq.slice original_s 0 (max * blocksize) in
+    Math.Lemmas.lemma_mult_le_right blocksize (i+1) max;
+    let block = FStar.Seq.slice original_s (i*blocksize) ((i+1)*blocksize) in
+    let r1 = FStar.Seq.append acc (f i block) in
+    assert (r1 == Seq.map_blocks_f blocksize max slice_s f i acc);
+
+    let idx_start = blocksize * i in
+    let out_len = seq_chunk_len updated_s blocksize i in
+    let new_block = f i (seq_get_exact_chunk updated_s blocksize i) in
+    assert (Seq.equal block (seq_get_exact_chunk updated_s blocksize i));
+    assert (f i block == new_block);
+
+    let r2 = Seq.update_sub updated_s idx_start out_len new_block in
+    assert (seq_chunk_len updated_s blocksize i == (
+      if blocksize * (i + 1) > Seq.length updated_s
+      then (if blocksize * i < Seq.length updated_s
+            then sub_rem_lemma i (Seq.length updated_s) blocksize;
+            Seq.length updated_s % blocksize)
+      else blocksize
+    ));
+    let proof_r2 (k:nat{(0 <= k /\ k < idx_start) \/ (idx_start + out_len <= k /\ k < len)}): Lemma (Seq.index r2 k == Seq.index updated_s k) = () in
+    assert (seq_set_exact_chunk #_ #len updated_s blocksize i new_block == r2);
+    let proof (j:nat{j < (i+1) * blocksize})
+      : Lemma (FStar.Seq.index r1 j == FStar.Seq.index r2 j)
+      = if j >= i * blocksize
+        then (
+          assert (FStar.Seq.index r1 j == FStar.Seq.index (f i block) (j - i * blocksize));
+          assert (FStar.Seq.index r2 j == FStar.Seq.index (f i (seq_get_exact_chunk updated_s blocksize i)) (j - i * blocksize));
+          assert (FStar.Seq.index r1 j == FStar.Seq.index r2 j)
+        ) else (
+          assert (FStar.Seq.index r1 j == FStar.Seq.index acc j);
+          assert (FStar.Seq.index r1 j == FStar.Seq.index updated_s j);
+          assert (i < max /\ max * blocksize <= len);
+          assert ((i+1) * blocksize <= len ==> j < len);
+          assert (j < len);
+          assert (j < idx_start);
+          proof_r2 j;
+          assert (FStar.Seq.index r2 j == FStar.Seq.index updated_s j);
+          // FStar.Seq.lemma_index_slice updated_s 0 (i * blocksize) j;
+          // assert (FStar.Seq.index (FStar.Seq.slice updated_s 0 (i * blocksize)) j == FStar.Seq.index updated_s (j + 0));
+          // assert (FStar.Seq.index acc j == FStar.Seq.index original_s (j + 0));
+          // assert (FStar.Seq.index updated_s j == FStar.Seq.index original_s j);
+          assert (FStar.Seq.index r1 j == FStar.Seq.index r2 j);
+          ()
+        )
+    in
+    FStar.Classical.forall_intro proof
+#pop-options
+
+
+
+// #push-options "--z3rlimit 100"
+// let map_blocks_f_equiv_lemma
+//   (len: uint_size) (blocksize: size_pos)
+//   (max: uint_size {max * blocksize <= len})
+//   (original_s: lseq 'a len)
+//   (f:(i:nat{i < max}) -> lseq 'a blocksize -> lseq 'a blocksize)
+//   (i: nat{i < max})
+//   (acc: lseq 'a (i * blocksize) {Seq.equal acc (FStar.Seq.slice s0 0 (i * blocksize))})
+//   : Lemma (
+//           let slice_s = FStar.Seq.slice s0 0 (max * blocksize) in
+//           forall (j: nat{j < (i+1) * blocksize}).
+//             FStar.Seq.index (Seq.map_blocks_f blocksize max slice_s f i acc) j
+//          == FStar.Seq.index (seq_set_exact_chunk #_ #len s0 blocksize i (f i (seq_get_exact_chunk s0 blocksize i))) j
+//     )
+//   = let slice_s = FStar.Seq.slice s0 0 (max * blocksize) in
+//     Math.Lemmas.lemma_mult_le_right blocksize (i+1) max;
+//     let block = FStar.Seq.slice s0 (i*blocksize) ((i+1)*blocksize) in
+//     let r1 = FStar.Seq.append acc (f i block) in
+//     assert (r1 == Seq.map_blocks_f blocksize max slice_s f i acc);
+
+//     let idx_start = blocksize * i in
+//     let out_len = seq_chunk_len s0 blocksize i in
+//     let new_block = f i (seq_get_exact_chunk s0 blocksize i) in
+//     let r2 = Seq.update_sub s0 idx_start out_len new_block in
+//     assert (seq_chunk_len s0 blocksize i == (
+//       if blocksize * (i + 1) > Seq.length s0
+//       then (if blocksize * i < Seq.length s0
+//             then sub_rem_lemma i (Seq.length s0) blocksize;
+//             Seq.length s0 % blocksize)
+//       else blocksize
+//     ));
+//     let proof_r2 (k:nat{(0 <= k /\ k < idx_start) \/ (idx_start + out_len <= k /\ k < len)}): Lemma (Seq.index r2 k == Seq.index s0 k) = () in
+//     assert (seq_set_exact_chunk #_ #len s0 blocksize i new_block == r2);
+//     let proof (j:nat{j < (i+1) * blocksize})
+//       : Lemma (FStar.Seq.index r1 j == FStar.Seq.index r2 j)
+//       = if j >= i * blocksize
+//         then (
+//           assert (FStar.Seq.index r1 j == FStar.Seq.index (f i block) (j - i * blocksize));
+//           assert (FStar.Seq.index r2 j == FStar.Seq.index (f i block) (j - i * blocksize));
+//           assert (FStar.Seq.index r1 j == FStar.Seq.index r2 j)
+//         ) else (
+//           assert (FStar.Seq.index r1 j == FStar.Seq.index acc j);
+//           assert (FStar.Seq.index r1 j == FStar.Seq.index s0 j);
+//           assert (i < max /\ max * blocksize <= len);
+//           assert ((i+1) * blocksize <= len ==> j < len);
+//           assert (j < len);
+//           assert (j < idx_start);
+//           proof_r2 j;
+//           assert (FStar.Seq.index r2 j == FStar.Seq.index s0 j);
+//           assert (FStar.Seq.index r1 j == FStar.Seq.index r2 j);
+//           ()
+//         )
+//     in
+//     FStar.Classical.forall_intro proof
+// #pop-options
+
+let map_blocks_foldi_fun
+  (len: uint_size) (blocksize: size_pos)
+  (max: uint_size {max * blocksize <= len})
+  (f:(i:nat{i < max}) -> lseq 'a blocksize -> lseq 'a blocksize)
+  = fun i (s: lseq 'a len) -> seq_set_exact_chunk #_ #len s blocksize i (f i (seq_get_exact_chunk s blocksize i))
+
+let map_blocks_foldi
+    (len: uint_size) (blocksize: size_pos)
+    (max: uint_size {max * blocksize <= len})
+    (n: uint_size {n * blocksize <= len /\ n <= max})
+    (s: lseq 'a len)
+    (f:(i:nat{i < max}) -> lseq 'a blocksize -> lseq 'a blocksize)
+    : lseq 'a len
+  = foldi 0 n (map_blocks_foldi_fun len blocksize max f) s
+
+#push-options "--z3rlimit 40"
+let rec map_blocks_foldi_preserves
+    (len: uint_size) (blocksize: size_pos)
+    (max: uint_size {max * blocksize <= len})
+    (n: uint_size {n * blocksize <= len /\ n <= max})
+    (s0: lseq 'a len)
+    (f:(i:nat{i < max}) -> lseq 'a blocksize -> lseq 'a blocksize)
+  : Lemma (
+      (forall (i:nat{i >= blocksize * n /\ i < len}). FStar.Seq.index s0 i == FStar.Seq.index (map_blocks_foldi len blocksize max n s0 f) i)
+    ) =
+      if n = 0
+      then unfold_foldi 0 n (map_blocks_foldi_fun len blocksize max f) s0
+      else (
+        unfold_left_foldi 0 n (map_blocks_foldi_fun len blocksize max f) s0;
+        assert (
+             map_blocks_foldi_fun len blocksize max f (n - 1) (map_blocks_foldi len blocksize max (n - 1) s0 f)
+          == map_blocks_foldi len blocksize max n s0 f
+        );
+        map_blocks_foldi_preserves len blocksize max (n - 1) s0 f;
+        admit ()
+      )
+#pop-options
+
+#push-options "--print_implicits"
+let direct_statement
+    (len: uint_size) (blocksize: size_pos)
+    (max: uint_size {max * blocksize <= len})
+    (n: uint_size {n * blocksize <= len /\ n <= max})
+    (s: lseq 'a len)
+    (f:(i:nat{i < max}) -> lseq 'a blocksize -> lseq 'a blocksize)
+  = let slice_s = FStar.Seq.slice s 0 (max * blocksize) in
+    let r1: Seq.map_blocks_a 'a blocksize max n = LC.repeat_gen n (Seq.map_blocks_a 'a blocksize max) (Seq.map_blocks_f blocksize max slice_s f) FStar.Seq.empty in
+    // let r2 = foldi 0 n (fun i (s: lseq 'a len) -> seq_set_exact_chunk #_ #len s blocksize i (f i (seq_get_exact_chunk s blocksize i))) s in
+    let r2 = map_blocks_foldi len blocksize max n s f in
+    (forall (i:nat{i < blocksize * n}). FStar.Seq.index r1 i == FStar.Seq.index r2 i)
+
+// #push-options "--fuel 0 --ifuel 0 --z3rlimit 150 --split_queries"
+#push-options "--fuel 0 --ifuel 0 --z3rlimit 50"
+let rec direct
+  (len: uint_size) (blocksize: size_pos)
+  (max: uint_size {max * blocksize <= len})
+  (n: uint_size {n * blocksize <= len /\ n <= max})
+  (s: lseq 'a len)
+  (f:(i:nat{i < max}) -> lseq 'a blocksize -> lseq 'a blocksize)
+  : Lemma (ensures (
+      direct_statement len blocksize max n s f
+      // let slice_s = FStar.Seq.slice s 0 (max * blocksize) in
+      // let r1: Seq.map_blocks_a 'a blocksize max n = LC.repeat_gen n (Seq.map_blocks_a 'a blocksize max) (Seq.map_blocks_f blocksize max slice_s f) FStar.Seq.empty in
+      // true
+      // let r2 = foldi 0 n (fun i (s: lseq 'a len) -> seq_set_exact_chunk #_ #len s blocksize i (f i (seq_get_exact_chunk s blocksize i))) s in
+      // let r2 = map_blocks_foldi len blocksize max n s f in
+      // forall (i:nat{i < blocksize * n}). FStar.Seq.index r1 i == FStar.Seq.index r2 i
+    )) (decreases n)
+  = if n = 0
+    then ()
+    else begin
+      let n': uint_size = n - 1 in
+      let slice_s = FStar.Seq.slice s 0 (max * blocksize) in
+      
+      let r1': s:seq 'a{Seq.length s == (n - 1) * blocksize} = LC.repeat_gen (n-1) (Seq.map_blocks_a 'a blocksize max) (Seq.map_blocks_f blocksize max slice_s f) FStar.Seq.empty in
+      // let r2' = foldi 0 (n-1) (fun i (s: lseq 'a len) -> seq_set_exact_chunk #_ #len s blocksize i (f i (seq_get_exact_chunk s blocksize i))) s in
+      let r2' = map_blocks_foldi len blocksize max (n - 1) s f in
+      let all1 = Seq.map_blocks_f blocksize max slice_s f (n-1) r1' in
+      let all2 = seq_set_exact_chunk #_ #len r2' blocksize (n-1) (f (n-1) (seq_get_exact_chunk r2' blocksize (n-1))) in
+      // let _ =
+        let _: squash (forall (i:nat{i < blocksize * (n - 1)}). FStar.Seq.index r1' i == FStar.Seq.index r2' i)
+          = assert_norm (direct_statement len blocksize max (n - 1) s f == (forall (i:nat{i < blocksize * (n - 1)}). FStar.Seq.index r1' i == FStar.Seq.index r2' i));
+            direct len blocksize max (n - 1) s f
+        in
+        map_blocks_foldi_preserves len blocksize max (n-1) s f;
+        map_blocks_f_equiv_lemma len blocksize max s f (n-1) r2' r1';
+        assert (forall (j: nat{j < n * blocksize}). FStar.Seq.index all1 j == FStar.Seq.index all2 j);
+      unfold_left_foldi 0 n (map_blocks_foldi_fun len blocksize max f) s;
+      // unfold_left_foldi 0 n (fun i (s: lseq 'a len) -> seq_set_exact_chunk #_ #len s blocksize i (f i (seq_get_exact_chunk s blocksize i))) s;
+      LC.unfold_repeat_gen n (Seq.map_blocks_a 'a blocksize max) (Seq.map_blocks_f blocksize max slice_s f) FStar.Seq.empty (n - 1);
+        ()
+    end
+#pop-options
+
+
+
+
+
+
+
+
+
+
+
+
+
+
+
+
+
+
+
+
+let direct_statement
+    (len: uint_size) (blocksize: size_pos)
+    (max: uint_size {max * blocksize <= len})
+    (n: uint_size {n * blocksize <= len /\ n <= max})
+    (s: lseq 'a len)
+    (f:(i:nat{i < max}) -> lseq 'a blocksize -> lseq 'a blocksize)
+  = let slice_s = FStar.Seq.slice s 0 (max * blocksize) in
+    let r1: Seq.map_blocks_a 'a blocksize max n = LC.repeat_gen n (Seq.map_blocks_a 'a blocksize max) (Seq.map_blocks_f blocksize max slice_s f) FStar.Seq.empty in
+    let r2 = foldi 0 n (fun i (s: lseq 'a len) -> seq_set_exact_chunk #_ #len s blocksize i (f i (seq_get_exact_chunk s blocksize i))) s in
+    (forall (i:nat{i < blocksize * n}). FStar.Seq.index r1 i == FStar.Seq.index r2 i)
+
+#push-options "--fuel 0 --ifuel 0 --z3rlimit 150 --split_queries"
+let rec direct
+  (len: uint_size) (blocksize: size_pos)
+  (max: uint_size {max * blocksize <= len})
+  (n: uint_size {n * blocksize <= len /\ n <= max})
+  (s: lseq 'a len)
+  (f:(i:nat{i < max}) -> lseq 'a blocksize -> lseq 'a blocksize)
+  : Lemma (ensures (
+      direct_statement len blocksize max n s f
+      // let slice_s = FStar.Seq.slice s 0 (max * blocksize) in
+      // let r1: Seq.map_blocks_a 'a blocksize max n = LC.repeat_gen n (Seq.map_blocks_a 'a blocksize max) (Seq.map_blocks_f blocksize max slice_s f) FStar.Seq.empty in
+      // true
+      // let r2 = foldi 0 n (fun i (s: lseq 'a len) -> seq_set_exact_chunk #_ #len s blocksize i (f i (seq_get_exact_chunk s blocksize i))) s in
+      // let r2 = map_blocks_foldi len blocksize max n s f in
+      // forall (i:nat{i < blocksize * n}). FStar.Seq.index r1 i == FStar.Seq.index r2 i
+    )) (decreases n)
+  = if n = 0
+    then ()
+    else begin
+      let n': uint_size = n - 1 in
+      let slice_s = FStar.Seq.slice s 0 (max * blocksize) in
+      // unfold_left_foldi 0 n (fun i (s: lseq 'a len) -> seq_set_exact_chunk #_ #len s blocksize i (f i (seq_get_exact_chunk s blocksize i))) s;
+      // LC.unfold_repeat_gen n (Seq.map_blocks_a 'a blocksize max) (Seq.map_blocks_f blocksize max slice_s f) FStar.Seq.empty (n - 1);
+      
+      let r1': s:seq 'a{Seq.length s == (n - 1) * blocksize} = LC.repeat_gen (n-1) (Seq.map_blocks_a 'a blocksize max) (Seq.map_blocks_f blocksize max slice_s f) FStar.Seq.empty in
+      let r2' = foldi 0 (n-1) (fun i (s: lseq 'a len) -> seq_set_exact_chunk #_ #len s blocksize i (f i (seq_get_exact_chunk s blocksize i))) s in
+      let all1 = Seq.map_blocks_f blocksize max slice_s f (n-1) r1' in
+      let all2 = seq_set_exact_chunk #_ #len r2' blocksize (n-1) (f (n-1) (seq_get_exact_chunk r2' blocksize (n-1))) in
+      let _ =
+        let _: squash (forall (i:nat{i < blocksize * (n - 1)}). FStar.Seq.index r1' i == FStar.Seq.index r2' i)
+          = assert_norm (direct_statement len blocksize max (n - 1) s f == (forall (i:nat{i < blocksize * (n - 1)}). FStar.Seq.index r1' i == FStar.Seq.index r2' i));
+            direct len blocksize max (n - 1) s f
+        in
+        map_blocks_foldi_preserves len blocksize max (n-1) s f;
+        map_blocks_f_equiv_lemma len blocksize max s f (n-1) r2' r1';
+        assert (
+          let slice_s = FStar.Seq.slice s 0 (max * blocksize) in
+            forall (j: nat{j < n * blocksize}).
+             FStar.Seq.index all1 j
+          == FStar.Seq.index all2 j
+        );
+        ()
+      in
+      // admitP ( Seq.map_blocks_f blocksize max slice_s f (n - 1) r1'
+      //       == seq_set_exact_chunk #_ #len s blocksize (n - 1) (f (n - 1) (seq_get_exact_chunk s blocksize (n - 1)))
+      // );
+      admit ()
+    end
+#pop-options
+
+//   (len: uint_size)
+//   (blocksize: size_pos)
+//   (i: nat {i < blocksize / len})
+//   (inp: lseq 'a len)
+//   (f:(i:nat{i < max} -> lseq 'a blocksize -> lseq 'a blocksize))
+//   : Lemma (ensures (
+//     forall (i: nat {i < len})
+//     // Math.Lemmas.cancel_mul_div n blocksize;
+//     // // assert (n <= max ==> Lib.Sequence.length inp == max * blocksize ==> range (n * blocksize) U32);
+//     // admitP (range (n * blocksize) U32);
+//     // map_blocks_pointwise_spec (n * blocksize) blocksize
+//     //                           (fun i ->
+//     //                             f i (seq_get_exact_chunk inp blocksize i)
+//     //                           )
+//     //                           FStar.Seq.empty
+//     //                           (LC.repeat_gen n (Seq.map_blocks_a 'a blocksize max) (Seq.map_blocks_f blocksize max inp f) FStar.Seq.empty)
+//   ))
+
+
+
+
+
+
+
+
+
+
+
+
+
+
+
+#push-options "--z3rlimit 200"
+let map_blocks_multi_repeat_gen_lemma_pointwise_spec
+  (blocksize:size_pos)
+  (max: nat)
+  (n: nat {n <= max})
+  (inp: seq 'a {Lib.Sequence.length inp == max * blocksize})
+  (f:(i:nat{i < max} -> lseq 'a blocksize -> lseq 'a blocksize))
+  : Lemma (ensures (
+    Math.Lemmas.cancel_mul_div n blocksize;
+    // assert (n <= max ==> Lib.Sequence.length inp == max * blocksize ==> range (n * blocksize) U32);
+    admitP (range (n * blocksize) U32);
+    map_blocks_pointwise_spec (n * blocksize) blocksize
+                              (fun i ->
+                                f i (seq_get_exact_chunk inp blocksize i)
+                              )
+                              FStar.Seq.empty
+                              (LC.repeat_gen n (Seq.map_blocks_a 'a blocksize max) (Seq.map_blocks_f blocksize max inp f) FStar.Seq.empty)
+  ))
+  = let r = LC.repeat_gen n (Seq.map_blocks_a 'a blocksize max) (Seq.map_blocks_f blocksize max inp f) FStar.Seq.empty in
+    if n = 0
+    then
+      admit ()
+      // map_blocks_pointwise_spec'0 0 blocksize
+      //                         (fun i ->
+      //                           f i (seq_get_exact_chunk inp blocksize i)
+      //                         )
+      //                         FStar.Seq.empty
+      //                         (LC.repeat_gen n (Seq.map_blocks_a 'a blocksize max) (Seq.map_blocks_f blocksize max inp f) FStar.Seq.empty)
+    else (
+      let n': nat = n - 1 in
+      LC.unfold_repeat_gen max (Seq.map_blocks_a 'a blocksize max) (Seq.map_blocks_f blocksize max inp f) FStar.Seq.empty n';
+      let acc = LC.repeat_gen n' (Seq.map_blocks_a 'a blocksize max) (Seq.map_blocks_f blocksize max inp f) FStar.Seq.empty in
+      Math.Lemmas.lemma_mult_le_right blocksize (n'+1) max;
+      let block = FStar.Seq.slice inp (n'*blocksize) ((n'+1)*blocksize) in
+      let result = FStar.Seq.append acc (f n' block) in
+      introduce forall k. FStar.Seq.index (FStar.Seq.slice inp (n'*blocksize) ((n'+1)*blocksize)) k == FStar.Seq.index inp (k + (n'*blocksize))
+           with FStar.Seq.lemma_index_slice inp (n'*blocksize) ((n'+1)*blocksize) k;
+      introduce forall (i:nat{i < (n'+1)*blocksize}). FStar.Seq.index result i == (if i < n' * blocksize
+                                                                            then FStar.Seq.index acc i
+                                                                            else FStar.Seq.index (f n' block) (i - n' * blocksize)
+                                                                            )
+           with begin
+                  if i < n' * blocksize 
+                  then FStar.Seq.lemma_index_app1 acc (f n' block) i
+                  else FStar.Seq.lemma_index_app2 acc (f n' block) i
+                end;
+      assert (r == result);
+      ()
+    )
+#pop-options
+
+#push-options "--z3rlimit 50"
+let map_blocks_multi_lemma_pointwise_spec
+  (blocksize:size_pos)
+  (max: nat)
+  (n: nat {n <= max})
+  (inp: seq 'a {Lib.Sequence.length inp == max * blocksize})
+  (f:(i:nat{i < max} -> lseq 'a blocksize -> lseq 'a blocksize))
+  : Lemma (ensures (
+    Math.Lemmas.cancel_mul_div n blocksize;
+    map_blocks_pointwise_spec (n * blocksize) blocksize
+                              (fun i ->
+                                f i (seq_get_exact_chunk inp blocksize i)
+                              )
+                              FStar.Seq.empty
+                              (Seq.map_blocks_multi blocksize max n inp f)
+  ))
+  = Seq.lemma_map_blocks_multi blocksize max n inp f;
+    let r' = Seq.map_blocks_multi blocksize max n inp f in
+    let r = LC.repeat_gen n (Seq.map_blocks_a 'a blocksize max) (Seq.map_blocks_f blocksize max inp f) FStar.Seq.empty in
+    map_blocks_multi_repeat_gen_lemma_pointwise_spec blocksize max n inp f
+#pop-options
+
+
+#push-options "--z3rlimit 500 --split_queries"
+let map_blocks_lemma_pointwise_spec
+  (#len: uint_size)
+  (blocksize:size_pos)
+  (inp:lseq 'a len)
+  (f:(Seq.block len blocksize -> lseq 'a blocksize -> lseq 'a blocksize))
+  (g:(Seq.last len blocksize -> rem:size_nat{rem < blocksize} -> s:lseq 'a rem -> lseq 'a rem))
+  : Lemma (
+    // true
+    map_blocks_pointwise_spec len blocksize
+                              (fun i -> f i (seq_get_exact_chunk inp blocksize i))
+                              (g (len / blocksize)
+                                 (len % blocksize)
+                                 (seq_get_remainder_chunk_length_lemma inp blocksize;
+                                  seq_get_remainder_chunk inp blocksize)
+                              )
+                              (Seq.map_blocks blocksize inp f g)
+  )
+  = Seq.lemma_map_blocks blocksize inp f g;
+    let len = Lib.Sequence.length inp in
+    let nb = len / blocksize in
+    let rem = len % blocksize in
+    let blocks = FStar.Seq.slice inp 0 (nb * blocksize) in
+    let last = FStar.Seq.slice inp (nb * blocksize) len in
+    Math.Lemmas.cancel_mul_div nb blocksize;
+    let bs = Lib.Sequence.map_blocks_multi #'a blocksize nb nb blocks f in
+    let res = if (rem > 0) then FStar.Seq.append bs (g nb rem last) else bs in
+    assert (res == Seq.map_blocks #'a blocksize inp f g);
+    ()
+  #pop-options
+
+
+#push-options "--z3rlimit 160"
+let s_chacha20_update' (ctx: S.state) (cipher: seq (int_t U8 SEC)): (r:seq _{r==s_chacha20_update ctx cipher}) =
+  Seq.lemma_map_blocks 64 cipher (S.chacha20_encrypt_block ctx) (S.chacha20_encrypt_last ctx);
+  let len = Seq.length cipher in
+  let nb  = len / 64 in
+  let rem = len % 64 in
+  let blocks = Seq.slice #_ #(seq_len cipher) cipher 0 (nb * 64) in
+  let last   = Seq.slice #_ #(seq_len cipher) cipher (nb * 64) len in
+  Math.Lemmas.cancel_mul_div nb 64;
+  let bs: seq _ = Seq.map_blocks_multi 64 nb nb blocks (S.chacha20_encrypt_block ctx) in
+
+  let aux (i: nat {i < nb * 64}): Lemma (
+      Seq.div_mul_lt 64 i nb;
+      let j = i / 64 in
+      let block: lseq (int_t U8 SEC) 64 = Seq.slice blocks (j * 64) ((j + 1) * 64) in
+      Seq.index #_ #(nb * 64) bs i == Seq.index (S.chacha20_encrypt_block ctx j block) (i % 64)
+  ) =
+      Seq.div_mul_lt 64 i nb;
+      Seq.index_map_blocks_multi 64 nb nb blocks (S.chacha20_encrypt_block ctx) i
+  in
+
+  FStar.Seq.append_empty_r bs;
+  let r = FStar.Seq.append bs (S.chacha20_encrypt_last ctx nb rem last) in
+  assert (r==s_chacha20_update ctx cipher);
+  // Classical.forall_intro aux;
+  r
+#pop-options
+
+
+
+let chacha20_update_ (st0 : state_t) (cipher : byte_seq) : r:byte_seq{r == chacha20_update st0 cipher} =
+  let blocks_out: seq uint8 = seq_new_ (secret (pub_u8 0x0)) (seq_len cipher) in
+  let n_blocks: uint_size = seq_num_exact_chunks cipher 64 in
+  let f (i: nat {i<n_blocks}): block_t = 
+    let msg_block: seq uint8 = seq_get_exact_chunk cipher 64 i in
+    chacha20_encrypt_block st0 (secret (pub_u32 i)) (array_from_seq 64 msg_block)
+  in
+  let blocks_out = IC.map_blocks_foldi'0 64 0 n_blocks f blocks_out in
+  let last_block: seq uint8 = seq_get_remainder_chunk cipher 64 in
+  if seq_len last_block <> 0 then
+    let b : seq uint8 = chacha20_encrypt_last st0 (secret (pub_u32 n_blocks)) last_block in
+    seq_set_chunk (blocks_out <: lseq _ (seq_len cipher)) 64 n_blocks b
+  else blocks_out
+
